tests/tactics/Hacl.Meta.fst
@@ -11,14 +11,14 @@ let tm_unit = `()
 [@@plugin]
 let mk (nm:string) (msg:string) : Tac (list sigelt) =
   let quote_string (s:string) : term =
-    pack_ln (Tv_Const (C_String s))
+    pack (Tv_Const (C_String s))
   in
-  let se = pack_sigelt (Sg_Let false [
-    pack_lb {
+  let se = pack_sigelt (Sg_Let {isrec=false;lbs=[
+    {
       lb_fv = pack_fv (cur_module () @ [nm]);
       lb_us = [];
       lb_typ = `int;
       lb_def = `(let x : unit = _ by (print (`#(quote_string msg)); exact tm_unit) in 42)
     }
-  ]) in
+  ]}) in
   [se]
